finished boogie implementation

sv_boogie.bpl
@@ -40,7 +40,6 @@ procedure sort() returns (perm : [int]int)
  
 }
 
-
 procedure qsPartition(lo : int, hi : int) returns (pivot_index: int, perm: [int]int) 
   modifies a_qs;
   requires lo <= hi;
@@ -113,74 +112,6 @@ procedure qsPartition(lo : int, hi : int) returns (pivot_index: int, perm: [int]
 
 }
 
-
-procedure qs(lo : int, hi : int) returns (perm: [int]int) 
-  modifies a_qs;
-  requires lo <= hi;
-  
-  // perm is a permutation
-  ensures (forall i: int :: lo <= i && i <= hi ==> lo <= perm[i] && perm[i] <= hi);
-  ensures (forall k, l: int :: lo <= k && k < l && l <= hi ==> perm[k] != perm[l]);
-  // the final array is that permutation of the input array
-  ensures (forall i: int :: lo <= i && i <= hi ==> a_qs[i] == old(a_qs)[perm[i]]);
-  
-  // array is sorted
-  ensures (forall k, l: int :: lo <= k && k <= l && l <= hi ==> a_qs[k] <= a_qs[l]);
-  
-  // rest of the array is untouched
-  ensures (forall k: int :: k < lo || k > hi ==> a_qs[k] == old(a_qs)[k]);
-{
-   // local variables
-  var n, pivot_index: int;
-  var perm_comb, perm_left, perm_right: [int]int;
-
-  if(lo < hi) {
-    call pivot_index, perm := qsPartition(lo,hi);
-    
-    // we have a non empty left part
-    if(lo < pivot_index) {
-      call perm_left := qs(lo, pivot_index - 1);
-      n := lo;
-      while(n < pivot_index) 
-        invariant lo <= n && n <= pivot_index;
-        invariant (forall i: int :: lo <= i && i < n ==> perm_comb[i] == perm_left[i]);
-        invariant (forall i: int :: lo <= i && i < n ==> lo <= perm_comb[i] && perm_comb[i] < pivot_index);
-        invariant (forall k, l: int :: lo <= k && k < l && l < n ==> perm_comb[k] != perm_comb[l]);
-      { perm_comb[n] := perm_left[n]; }
-     
-    }     
-    
-    // we have a non empty right part
-    if(pivot_index + 1 <= hi) {
-      call perm_right := qs(pivot_index + 1, hi);
-      n := pivot_index + 1;
-      while(n <= hi) 
-        invariant pivot_index + 1 <= n && n <= hi+1;
-        invariant (forall i: int :: pivot_index + 1 <= i && i < n ==> perm_comb[i] == perm_right[i]);
-        invariant (forall i: int :: pivot_index + 1 <= i && i < n ==> pivot_index + 1 <= perm_comb[i] && perm_comb[i] <= hi);
-        invariant (forall k, l: int :: pivot_index + 1 <= k && k < l && l < n ==> perm_comb[k] != perm_comb[l]);
-      { perm_comb[n] := perm_left[n]; }
-    }
-    
-    perm_comb[pivot_index] := pivot_index;
-    // perm_comb is now a permutation
-
-    // combine perm_comb with perm
-    n := lo;
-    while(n <= hi) 
-      invariant lo <= n && n <= hi+1;
-      invariant (forall i: int :: lo <= i && i < n ==> perm[i] == perm_comb[perm[i]]);
-      invariant (forall i: int :: lo <= i && i < n ==> lo <= perm[i] && perm[i] <= hi);
-      invariant (forall k, l: int :: lo <= k && k < l && l < n ==> perm[k] != perm[l]);
-      invariant (forall i: int :: lo <= i && i < n ==> a_qs[i] == old(a_qs)[perm[i]]);
-    { perm[n] := perm_comb[perm[n]]; }
-    
-  } else {
-    perm[lo] := lo;
-  }
-    
-}
-
 // public interface for quicksort that can be used to sort arbitrary arrays
 procedure quickSort(arr : [int]int, lo : int, hi : int) returns (arr_sorted : [int]int, perm: [int]int) 
   modifies a_qs;
@@ -202,24 +133,122 @@ procedure quickSort(arr : [int]int, lo : int, hi : int) returns (arr_sorted : [i
 }
 
 
-procedure bucketSort(lo : int, hi : int) returns (perm: [int]int)
-  modifies a,a_qs; //, b0, b1, b2;
-  // only allow bucketsort to be called from [0..N-1]
-  requires lo == 0;
-  requires hi == N-1;
+procedure qs(lo : int, hi : int) returns (perm: [int]int) 
+  modifies a_qs;
+  requires lo <= hi;
   // perm is a permutation
   ensures (forall i: int :: lo <= i && i <= hi ==> lo <= perm[i] && perm[i] <= hi);
   ensures (forall k, l: int :: lo <= k && k < l && l <= hi ==> perm[k] != perm[l]);
   // the final array is that permutation of the input array
-  ensures (forall i: int :: lo <= i && i <= hi ==> a[i] == old(a)[perm[i]]);
+  ensures (forall i: int :: lo <= i && i <= hi ==> a_qs[i] == old(a_qs)[perm[i]]);
+  // array is sorted
+  ensures (forall k, l: int :: lo <= k && k <= l && l <= hi ==> a_qs[k] <= a_qs[l]);
+  // rest of the array is untouched
+  ensures (forall k: int :: k < lo || k > hi ==> a_qs[k] == old(a_qs)[k]);
+{
+   // local variables
+  var n, pivot_index: int;
+  var perm_comb, perm_left, perm_right, perm_res: [int]int;
+  
+  if(lo < hi) {
+    call pivot_index, perm := qsPartition(lo,hi);
+    assert (forall i: int :: lo <= i && i <= hi ==> a_qs[i] == old(a_qs)[perm[i]]);
+
+    // we have a non empty left part
+    if(lo < pivot_index) {
+      call perm_left := qs(lo, pivot_index - 1);
+
+      n := lo;
+      while(n < pivot_index) 
+        invariant lo <= n && n <= pivot_index;
+        invariant (forall i: int :: lo <= i && i < n ==> perm_comb[i] == perm_left[i]);
+        invariant (forall i: int :: lo <= i && i < n ==> lo <= perm_comb[i] && perm_comb[i] <= hi);
+        invariant (forall k, l: int :: lo <= k && k < l && l < n ==> perm_comb[k] != perm_comb[l]);
+      { 
+        perm_comb[n] := perm_left[n];
+        n := n+1;
+      }
+    }     
+
+    //assert (forall i: int :: lo <= i && i <= pivot_index-1 ==> a_qs[i] == old(a_qs)[perm[perm_comb[i]]]);
+    //assert (forall i: int :: pivot_index + 1 <= i && i <= hi ==> a_qs[i] == old(a_qs)[perm[i]]);
+
+    // we have a non empty right part
+    if(pivot_index + 1 <= hi) {
+      call perm_right := qs(pivot_index + 1, hi);
+
+      n := pivot_index + 1;
+      while(n <= hi)
+        // maintain previous information about perm_comb
+          invariant (forall i: int :: lo <= i && i < pivot_index ==> perm_comb[i] == perm_left[i]);
+          invariant (forall i: int :: lo <= i && i < pivot_index ==> lo <= perm_comb[i] && perm_comb[i] <= hi);
+          invariant (forall k, l: int :: lo <= k && k < l && l < pivot_index ==> perm_comb[k] != perm_comb[l]);
+          invariant (forall i: int :: lo <= i && i <= pivot_index-1 ==> a_qs[i] == old(a_qs)[perm[perm_comb[i]]]);
+
+          invariant pivot_index + 1 <= n && n <= hi+1;
+          invariant (forall i: int :: pivot_index + 1 <= i && i < n ==> perm_comb[i] == perm_right[i]);
+          invariant (forall i: int :: pivot_index + 1 <= i && i < n ==> pivot_index + 1 <= perm_comb[i] && perm_comb[i] <= hi);
+          invariant (forall k, l: int :: pivot_index + 1 <= k && k < l && l < n ==> perm_comb[k] != perm_comb[l]);
+      { 
+        perm_comb[n] := perm_right[n]; 
+        n := n+1;
+      }
+    }
+
+    //assert (forall i: int :: pivot_index + 1 <= i && i <= hi ==> a_qs[i] == old(a_qs)[perm[perm_comb[i]]]);
+    //assert (forall i: int :: lo <= i && i <= pivot_index-1 ==> a_qs[i] == old(a_qs)[perm[perm_comb[i]]]);
+
+    perm_comb[pivot_index] := pivot_index;
+    // perm_comb is now a permutation
+
+    //assert (forall i: int :: lo <= i && i <= hi ==> lo <= perm[i] && perm[i] <= hi);
+    //assert (forall i: int :: lo <= i && i <= hi ==> lo <= perm_comb[i] && perm_comb[i] <= hi);
+
+    //IMPORTANT: without this assert the verify doesn't terminate
+    assert (forall k, l: int :: lo <= k && k <= l && l <= hi  ==> a_qs[k] <= a_qs[l]);
+
+    // combine perm_comb with perm
+    n := lo;
+    while(n <= hi) 
+      invariant lo <= n && n <= hi+1;
+      invariant (forall i: int :: lo <= i && i < n ==> perm_res[i] == perm[perm_comb[i]]);
+      invariant (forall i: int :: lo <= i && i < n ==> lo <= perm_res[i] && perm_res[i] <= hi);
+      invariant (forall k, l: int :: lo <= k && k < l && l < n ==> perm_res[k] != perm_res[l]);
+      invariant (forall i: int :: lo <= i && i <= hi ==> a_qs[i] == old(a_qs)[perm[perm_comb[i]]]);
+    { 
+      perm_res[n] := perm[perm_comb[n]];
+      n := n+1;  
+    }
+
+    // write updated permutation back to perm
+    perm := perm_res;
+    
+  } else {
+    perm[lo] := lo;
+  }
+
+  // IMPORTANT: this assert is crutial for boogie to terminate
+  assert (forall i: int :: lo <= i && i <= hi ==> a_qs[i] == old(a_qs)[perm[i]]);
+}
+
+
+procedure bucketSort(lo : int, hi : int) returns (perm: [int]int)
+  modifies a,a_qs; //, b0, b1, b2;
+  // only allow bucketsort to be called from [0..N-1]
+  requires 0 <= lo && lo <= hi;
+  // perm is a permutation
+  ensures (forall k: int :: lo <= k && k <= hi ==> lo <= perm[k] && perm[k] <= hi);
+  ensures (forall k, l: int :: lo <= k && k < l && l <= hi ==> perm[k] != perm[l]);
+  // the final array is that permutation of the input array
+  ensures (forall k: int :: lo <= k && k <= hi ==> a[k] == old(a)[perm[k]]);
   // array is sorted
   ensures (forall k, l: int :: lo <= k && k <= l && l <= hi  ==> a[k] <= a[l]);
 {
   
   //buckets' end indices
-  var b0_i:int;
-  var b1_i:int;
-  var b2_i:int;
+  var b0_i, off_b0:int;
+  var b1_i, off_b1:int;
+  var b2_i, off_b2:int;
   
   //buckets' upper bounds (exclusive)
   var bound_0:int;
@@ -228,6 +257,10 @@ procedure bucketSort(lo : int, hi : int) returns (perm: [int]int)
   
   //bucket permutations
   var perm0, perm1, perm2 : [int]int;
+  var permAtoB0 : [int]int;
+  var permAtoB1 : [int]int;
+  var permAtoB2 : [int]int;
+  var permA : [int]int;
 
   var b0, b0_sorted, b1, b1_sorted, b2, b2_sorted: [int]int;
   
@@ -245,91 +278,181 @@ procedure bucketSort(lo : int, hi : int) returns (perm: [int]int)
   while(i <= hi)
     invariant (i >= lo && i <= hi+1);
     // array 'a' is divided over b0,b1 and b2
-    invariant b0_i+b1_i+b2_i == lo+i;
-
+    invariant i-lo == b0_i+b1_i+b2_i; 
     //all buckets contain the correct kind of elements:
     invariant(forall e:int :: (e >= 0 && e < b0_i) ==> (b0[e] < -1*N));
     invariant(forall e:int :: (e >= 0 && e < b1_i) ==> (b1[e] >= -1*N && b1[e] < N));
     invariant(forall e:int :: (e >= 0 && e < b2_i) ==> (b2[e] >= N));
-        
-    {
-      
+    
+    //permAtoB holds the mapping of elements from A onto the buckets
+    invariant(forall e:int :: (e >= 0 && e < b0_i) ==> (b0[e] == a[permAtoB0[e]]));
+    invariant(forall e:int :: (e >= 0 && e < b1_i) ==> (b1[e] == a[permAtoB1[e]]));
+    invariant(forall e:int :: (e >= 0 && e < b2_i) ==> (b2[e] == a[permAtoB2[e]]));
+    
+    invariant (forall k: int :: 0 <= k && k < b0_i ==> lo <= permAtoB0[k] && permAtoB0[k] <= hi);
+    invariant (forall k: int :: 0 <= k && k < b1_i ==> lo <= permAtoB1[k] && permAtoB1[k] <= hi);
+    invariant (forall k: int :: 0 <= k && k < b2_i ==> lo <= permAtoB2[k] && permAtoB2[k] <= hi);
+    
+    //every element is permuted
+    invariant (forall k: int :: 0 <= k && k < b0_i ==> permAtoB0[k] < i);
+    invariant (forall k: int :: 0 <= k && k < b1_i ==> permAtoB1[k] < i);
+    invariant (forall k: int :: 0 <= k && k < b2_i ==> permAtoB2[k] < i);
+    
+    invariant(forall e,f : int :: ((e >= 0 && e < b0_i && e != f && f >= 0 && f < b0_i) ==> (permAtoB0[e] != permAtoB0[f])));
+    invariant(forall e,f : int :: ((e >= 0 && e < b1_i && e != f && f >= 0 && f < b1_i) ==> (permAtoB1[e] != permAtoB1[f])));
+    invariant(forall e,f : int :: ((e >= 0 && e < b2_i && e != f && f >= 0 && f < b2_i) ==> (permAtoB2[e] != permAtoB2[f])));
+    
+    invariant(forall e,f : int :: ((e >= 0 && e < b0_i && f >=0 && f < b1_i) ==> (permAtoB0[e] != permAtoB1[f])));
+    invariant(forall e,f : int :: ((e >= 0 && e < b0_i && f >=0 && f < b2_i) ==> (permAtoB0[e] != permAtoB2[f])));
+    invariant(forall e,f : int :: ((e >= 0 && e < b1_i && f >=0 && f < b2_i) ==> (permAtoB1[e] != permAtoB2[f])));
+  {
     //add a[i] to correct bucket
     if(a[i] < bound_1){
       if(a[i] < bound_0){
         b0[b0_i] := a[i];
+        permAtoB0[b0_i] := i;
+        
         b0_i := b0_i + 1;
       }
       else{
         b1[b1_i] := a[i];
+        permAtoB1[b1_i] := i;
+        
         b1_i := b1_i + 1;
       }
     }
     else{
       b2[b2_i] := a[i];
+      permAtoB2[b2_i] := i;
+        
       b2_i := b2_i + 1;
     }
-    
     i := i + 1;
   }
   
-  // sort first bucket if non-empty
-  if(b0_i > 0) { call b0_sorted, perm0 := quickSort(b0, 0, b0_i-1); }
-  // copy back elements from bucket to array
   i := 0;
   while(i < b0_i)
-    // copied values are sorted
-    invariant (forall k: int :: 0 <= k && k < i ==> a[k+lo] == b0_sorted[k]);
-    invariant (forall k, l: int :: 0 <= k && k <= l && l < i ==> a[k+lo] <= a[l+lo]);
+    invariant (i >= 0 && i <= b0_i);
+    invariant(forall e:int :: (e >= 0 && e < i) ==> (b0[e] == a[permA[e]]));
+    invariant (forall k: int :: 0 <= k && k < i ==> lo <= permA[k] && permA[k] <= hi);
+    
+    invariant (forall e:int :: (e >=0 && e < i ==> permA[e] == permAtoB0[e]));
+    invariant (forall e,f:int :: (e >= 0 && e < f && f < i ==> permA[e] != permA[f]));
   {
-    a[i+lo] := b0_sorted[i];
+    permA[i] := permAtoB0[i];
     i := i + 1;
   }
   
-  // sort second bucket if non-empty
-  if(b1_i > 0) { call b1_sorted, perm1 := quickSort(b1, 0, b1_i-1); }
-  // copy back elements from bucket to array
-
   i := 0;
   while(i < b1_i)
-    // preserve info. about first part of array
-    invariant (forall k: int :: 0 <= k && k < b0_i ==> a[k+lo] == b0_sorted[k]);
-    invariant (forall k, l: int :: 0 <= k && k <= l && l < b0_i ==> a[k+lo] <= a[l+lo]);
+    invariant(i >= 0 && i <= b1_i);
+    invariant(forall e:int :: (e >= 0 && e < b0_i) ==> (b0[e] == a[permA[e]]));
+    invariant(forall e:int :: (e >= 0 && e < i) ==> (b1[e] == a[permA[e + b0_i]]));
+    invariant (forall k: int :: 0 <= k && k < b0_i ==> lo <= permA[k] && permA[k] <= hi);
+    invariant (forall k: int :: b0_i <= k && k < i+b0_i ==> lo <= permA[k] && permA[k] <= hi);
     
-    // copied values are sorted
-    invariant (forall k: int :: 0 <= k && k < i ==> a[k+lo+b0_i] == b1_sorted[k]);
-    invariant (forall k, l: int :: 0 <= k && k <= l && l < i ==> a[k+lo+b0_i] <= a[l+lo+b0_i]);
-      
+    invariant(forall f:int :: (f >= b0_i && f < b0_i + i ==> permA[f] == permAtoB1[f-b0_i]));
+
+    invariant(forall e:int :: (e >= 0 && e < b0_i + i ==> (permA[e] == permAtoB0[e] || permA[e] == permAtoB1[e-b0_i])));
+    invariant (forall e,f:int :: (e >= 0 && e < i+ b0_i && e != f && f >= 0 && f < i + b0_i ==> permA[e] != permA[f]));
   {
-    a[i+lo+b0_i] := b1_sorted[i];   
+    permA[i+b0_i] := permAtoB1[i];
+    i := i + 1;
   }
   
-
-  // sort third bucket if non-empty
-  if(b2_i > 0) { call b2_sorted, perm2 := quickSort(b2, 0, b2_i-1); }
-  // copy back elements from bucket to array
   i := 0;
   while(i < b2_i)
-    // preserve info. about first part of array
-    invariant (forall k: int :: 0 <= k && k < b0_i ==> a[k+lo] == b0_sorted[k]);
-    invariant (forall k, l: int :: 0 <= k && k <= l && l < b0_i ==> a[k+lo] <= a[l+lo]);
+    invariant(i >= 0 && i <= b2_i);
+    invariant(forall e:int :: (e >= 0 && e < b0_i) ==> (b0[e] == a[permA[e]]));
+    invariant(forall e:int :: (e >= 0 && e < b1_i) ==> (b1[e] == a[permA[e + b0_i]]));
+    invariant(forall e:int :: (e >= 0 && e < i) ==> (b2[e] == a[permA[e + b0_i + b1_i]]));
+    invariant (forall k: int :: 0 <= k && k < b0_i ==> lo <= permA[k] && permA[k] <= hi);
+    invariant (forall k: int :: b0_i <= k && k < b1_i+b0_i ==> lo <= permA[k] && permA[k] <= hi);
+    invariant (forall k: int :: b0_i + b1_i <= k && k < b0_i + b1_i + i ==> lo <= permA[k] && permA[k] <= hi);
     
-    // preserve info. about second part of array
-    invariant (forall k: int :: 0 <= k && k < b1_i ==> a[k+lo+b0_i] == b1_sorted[k]);
-    invariant (forall k, l: int :: 0 <= k && k <= l && l < b1_i ==> a[k+lo+b0_i] <= a[l+lo+b0_i]);
+    invariant(forall f:int :: (f >= b0_i+b1_i && f < b0_i + b1_i + i ==> permA[f] == permAtoB2[f-b0_i-b1_i]));
+    invariant(forall e:int :: (e >= 0 && e < b0_i + b1_i + i ==> (permA[e] == permAtoB0[e] || permA[e] == permAtoB1[e-b0_i] || permA[e] == permAtoB2[e-b1_i-b0_i])));
     
-    // copied values are sorted
-    invariant (forall k: int :: 0 <= k && k < i ==> a[k+lo+b0_i+b1_i] == b2_sorted[k]);
-    invariant (forall k, l: int :: 0 <= k && k <= l && l < i ==> a[k+lo+b0_i+b1_i] <= a[l+lo+b0_i+b1_i]);
+    invariant (forall e,f:int :: (e >= 0 && e < b1_i+ b0_i && e != f && f >= 0 && f < b1_i + b0_i ==> permA[e] != permA[f]));
+    invariant (forall e,f:int :: (e >= 0 && e < i+ b1_i + b0_i && e != f && f >= 0 && f < i + b1_i + b0_i ==> permA[e] != permA[f]));
   {
-    a[i+lo+b0_i+b1_i] := b2_sorted[i];   
+    permA[i + b0_i + b1_i] := permAtoB2[i];
+    i := i + 1;
   }
   
-  //TODO prove that array is permutation of original
-  assume (forall k: int :: lo <= k && k <= hi ==> lo <= perm[k] && perm[k] <= hi);
-  assume (forall k, l: int :: lo <= k && k < l && l <= hi ==> perm[k] != perm[l]);
-  // the final array is that permutation of the input array
-  assume (forall k: int :: lo <= k && k <= hi ==> a[k] == old(a)[perm[k]]);
+  // index mapping from bucket indexes to array indexes 
+  off_b0 := lo + b0_i; // end index of bucket0 in a (exclusive)
+  off_b1 := lo + b0_i + b1_i; // end index of bucket1 in a (exclusive)
+  off_b2 := lo + b0_i + b1_i + b2_i; // end index of bucket2 in a (exclusive)
+  
+  // sort all buckets
+  if(b0_i > 0) { call b0_sorted, perm0 := quickSort(b0, 0, b0_i-1); }
+  if(b1_i > 0) { call b1_sorted, perm1 := quickSort(b1, 0, b1_i-1); }
+  if(b2_i > 0) { call b2_sorted, perm2 := quickSort(b2, 0, b2_i-1); }
 
+  i := lo;
+  while(i < off_b0)
+    // bucket values are copied to a
+    invariant (forall k: int :: lo <= k && k < i ==> a[k] == b0_sorted[k-lo]);
+    invariant (forall k: int :: lo <= k && k < i ==> a[k] == old(a[perm[k]]));
+    invariant (forall k: int :: lo <= k && k < i ==> lo <= perm[k] && perm[k] <= hi);
+    
+    invariant(forall f:int ::(f >= lo && f < i ==> perm[f] == permA[perm0[f-lo]]));
+    invariant(forall e,f:int :: (e >= lo && e < i && e != f && f >= lo && f < i ==> perm[e] != perm[f]));
+  {
+    a[i] := b0_sorted[i-lo];
+    perm[i] := permA[perm0[i-lo]];
+    i := i + 1;
+  }
+
+  // copy back elements from bucket to array
+  i := off_b0;
+  while(i < off_b1)
+    // needed to ensure that only this part of array is modified
+    invariant off_b0 <= i && i <= off_b1; 
+    // previous knowledge about a is preserved
+    invariant (forall k: int :: lo <= k && k < off_b0 ==> a[k] == b0_sorted[k-lo]);
+    // bucket values are copied to a
+    invariant (forall k: int :: off_b0 <= k && k < i ==> a[k] == b1_sorted[k-off_b0]);
+    
+    //permutation
+    invariant (forall k: int :: lo <= k && k < off_b0 ==> a[k] == old(a[perm[k]]));
+    invariant (forall k: int :: off_b0 <= k && k < i ==> a[k] == old(a[perm[k]]));
+    invariant (forall k: int :: lo <= k && k < off_b0 ==> lo <= perm[k] && perm[k] <= hi);
+    invariant (forall k: int :: off_b0 <= k && k < i ==> lo <= perm[k] && perm[k] <= hi);
+    
+    invariant(forall f:int ::(f >= off_b0 && f < i ==> perm[f] == permA[perm1[f-b0_i-lo] + b0_i]));
+    invariant(forall e,f:int :: (e >= lo && e < i && e != f && f >= lo && f < i ==> perm[e] != perm[f]));
+  {
+    a[i] := b1_sorted[i-off_b0];
+    perm[i] := permA[perm1[i-b0_i-lo] + b0_i];
+    i := i + 1;
+  }
+  
+  i := off_b1;
+  while(i < off_b2)
+    // needed to ensure that only this part of array is modified
+    invariant off_b1 <= i && i <= off_b2; 
+    // previous knowledge about a is preserved
+    invariant (forall k: int :: lo <= k && k < off_b0 ==> a[k] == b0_sorted[k-lo]);
+    invariant (forall k: int :: off_b0 <= k && k < off_b1 ==> a[k] == b1_sorted[k-off_b0]);
+    // bucket values are copied to a
+    invariant (forall k: int :: off_b1 <= k && k < i ==> a[k] == b2_sorted[k-off_b1]);
+    
+    //permutation
+    invariant (forall k: int :: lo <= k && k < off_b0 ==> a[k] == old(a[perm[k]]));
+    invariant (forall k: int :: off_b0 <= k && k < off_b1 ==> a[k] == old(a[perm[k]]));
+    invariant (forall k: int :: off_b1 <= k && k < i ==> a[k] == old(a[perm[k]]));
+    invariant (forall k: int :: lo <= k && k < off_b0 ==> lo <= perm[k] && perm[k] <= hi);
+    invariant (forall k: int :: off_b0 <= k && k < off_b1 ==> lo <= perm[k] && perm[k] <= hi);
+    invariant (forall k: int :: off_b1 <= k && k < i ==> lo <= perm[k] && perm[k] <= hi);
+    
+    invariant(forall f:int ::(f >= off_b1 && f < i ==> perm[f] == permA[perm2[f-b0_i-b1_i-lo] + b0_i + b1_i]));
+    invariant(forall e,f:int :: (e >= lo && e < i && e != f && f >= lo && f < i ==> perm[e] != perm[f]));
+  {
+    a[i] := b2_sorted[i-off_b1];
+    perm[i] := permA[perm2[i-b0_i-b1_i-lo] + b0_i + b1_i];
+    i := i + 1;
+  }
 }
 
